nozo/33-IMP-in-Coq/IMP-in-Coq.md
@@ -207,6 +207,322 @@ Proof.
 Qed.
 ```
 
+```coq
+(* Defining state *)
+
+Definition total_map (A : Type) := string -> A.
+
+Definition eqb_string (x y : string) : bool :=
+    if string_dec x y then true else false.
+
+Definition t_empty {A : Type} (v : A) : total_map A :=
+    (fun _ => v).
+
+Definition t_update {A : Type} (m : total_map A)
+                    (x : string) (v : A)
+                    : total_map A :=
+    fun x' => if (eqb_string x x') then v else m x'.
+
+Notation "'_' '!->' v" := (t_empty v)
+    (at level 100, right associativity).
+Notation "x '!->' v ';' m" := (t_update m x v)
+    (at level 100, v at next level, right associativity).
+
+Definition state := total_map nat.
+Definition empty_st := (_ !-> 0).
+Notation "x '!->' v" := (x !-> v ; empty_st)
+    (at level 100).
+```
+
+```coq
+Definition W : string := "W".
+Definition X : string := "X".
+Definition Y : string := "Y".
+Definition Z : string := "Z".
+
+Compute (X !-> 1; Y !-> 2) X.
+(*
+= 1
+: nat
+ *)
+```
+
+```coq
+(* Defining Syntax *)
+
+Inductive aexp : Type :=
+    | ANum : nat -> aexp
+    | AId : string -> aexp
+    | APlus : aexp -> aexp -> aexp
+    | AMinus : aexp -> aexp -> aexp
+    | AMult : aexp -> aexp -> aexp.
+
+Inductive bexp : Type :=
+    | BTrue : bexp
+    | BFalse : bexp
+    | BEq : aexp -> aexp -> bexp
+    | BLe : aexp -> aexp -> bexp
+    | BNot : bexp -> bexp
+    | BAnd : bexp -> bexp -> bexp.
+```
+
+```coq
+(* Defining Notation *)
+
+Coercion AId : string >-> aexp.
+Coercion ANum : nat >-> aexp.
+Declare Custom Entry com.
+Declare Scope com_scope.
+Notation "<{ e }>" := e (at level 0, e custom com at level 99) : com_scope.
+Notation "( x )" := x (in custom com, x at level 99) : com_scope.
+Notation "x" := x (in custom com at level 0, x constr at level 0) : com_scope.
+Notation "f x .. y" := (.. (f x) .. y)
+                  (in custom com at level 0, only parsing,
+                  f constr at level 0, x constr at level 9,
+                  y constr at level 9) : com_scope.
+Notation "x + y" := (APlus x y) (in custom com at level 50, left associativity).
+Notation "x - y" := (AMinus x y) (in custom com at level 50, left associativity).
+Notation "x * y" := (AMult x y) (in custom com at level 40, left associativity).
+Notation "'true'" := true (at level 1).
+Notation "'true'" := BTrue (in custom com at level 0).
+Notation "'false'" := false (at level 1).
+Notation "'false'" := BFalse (in custom com at level 0).
+Notation "x <= y" := (BLe x y) (in custom com at level 70, no associativity).
+Notation "x = y" := (BEq x y) (in custom com at level 70, no associativity).
+Notation "x && y" := (BAnd x y) (in custom com at level 80, left associativity).
+Notation "'~' b" := (BNot b) (in custom com at level 75, right associativity).
+Open Scope com_scope.
+
+Check <{ 3 + (X * 2) }>.
+(* 
+<{ 3 + X * 2 }>
+	 : aexp
+ *)
+```
+
+```coq
+(* Defining Evaluation as a function *)
+
+Fixpoint aeval (st : state) (a : aexp) : nat :=
+    match a with
+    | ANum n => n
+    | AId x => st x
+    | <{a1 + a2}> => (aeval st a1) + (aeval st a2)
+    | <{a1 - a2}> => (aeval st a1) - (aeval st a2)
+    | <{a1 * a2}> => (aeval st a1) * (aeval st a2)
+    end.
+
+Fixpoint beval (st : state) (b : bexp) : bool :=
+    match b with
+    | <{true}> => true
+    | <{false}> => false
+    | <{a1 = a2}> => (aeval st a1) =? (aeval st a2)
+    | <{a1 <= a2}> => (aeval st a1) <=? (aeval st a2)
+    | <{~ b1}> => negb (beval st b1)
+    | <{b1 && b2}> => andb (beval st b1) (beval st b2)
+    end.
+
+Compute aeval (X !-> 5) <{ 3 + (X * 2) }>.
+(* 
+= 13
+: nat
+ *)
+```
+
+```
+    c := skip
+      | x := a
+      | c ; c
+      | if b then c else c end
+      | while b do c end
+```
+
+```coq
+(* Defining Syntax *)
+
+Inductive com : Type :=
+    | CSkip : com
+    | CAsgn : string -> aexp -> com
+    | CSeq : com -> com -> com
+    | CIf : bexp -> com -> com -> com
+    | CWhile : bexp -> com -> com.
+```
+
+```coq
+(* Defining Notation *)
+
+Notation "'skip'" :=
+         CSkip (in custom com at level 0) : com_scope.
+Notation "x := y" :=
+         (CAsgn x y)
+            (in custom com at level 0, x constr at level 0,
+             y at level 85, no associativity) : com_scope.
+Notation "x ; y" :=
+         (CSeq x y)
+           (in custom com at level 90, right associativity) : com_scope.
+Notation "'if' x 'then' y 'else' z 'end'" :=
+         (CIf x y z)
+           (in custom com at level 89, x at level 99,
+            y at level 99, z at level 99) : com_scope.
+Notation "'while' x 'do' y 'end'" :=
+         (CWhile x y)
+            (in custom com at level 89, x at level 99, y at level 99) : com_scope.
+
+Definition fact_in_coq : com :=
+    <{
+        Z := X;
+        Y := 1;
+        while ~(Z = 0) do
+            Y := Y * Z;
+            Z := Z - 1
+        end
+    }>.
+```
+
+```coq
+(* Defining Evaluation as a function (Error) *)
+
+Fixpoint ceval (st : state) (c : com) : state :=
+    match c with
+        | <{ skip }> =>
+            st
+        | <{ x := a }> =>
+            (x !-> (aeval st a) ; st)
+        | <{ c1 ; c2 }> =>
+            let st' := ceval st c1 in
+            ceval st' c2
+        | <{ if b then c1 else c2 end}> =>
+            if (beval st b)
+            then ceval st c1
+            else ceval st c2
+        | <{ while b do c end }> =>
+            if (beval st b)
+            then ceval st <{ while b do c end }>
+            else st
+    end.
+
+(* 
+Cannot guess decreasing argument of fix.
+ *)
+```
+
+$$
+\frac{}{\verb+ st =[ skip ]=> st +}\ (ESkip)
+$$
+
+$$
+\frac{\verb+ aeval st a = n +}
+     {\verb+ st =[ x := a ]=> (x !-> n ; st) +}\ (EAsgn)
+$$
+
+$$
+\frac{\verb+ st =[ c1 ]=> st' +\qquad
+      \verb+ st' =[ c2 ]=> st'' +}
+     {\verb+ st =[ c1;c2 ]=> st'' +}\ (ESeq)
+$$
+
+$$
+\frac{\verb+ beval st b = true +\qquad
+      \verb+ st =[ c1 ]=> st' +}
+     {\verb+ st =[ if b then c1 else c2 end ]=> st' +}\ (EIfTrue)
+$$
+
+$$
+\frac{\verb+ beval st b = false +\qquad
+      \verb+ st =[ c2 ]=> st' +}
+     {\verb+ st =[ if b then c1 else c2 end ]=> st' +}\ (EIfFalse)
+$$
+
+$$
+\frac{\verb+ beval st b = false +}
+     {\verb+ st =[ while b do c end ]=> st +}\ (EWhileFalse)
+$$
+
+$$
+\frac{\verb+ beval st b = true +\qquad
+      \verb+ st =[ c ]=> st' +\qquad
+      \verb+ st' =[ while b do c end ]=> st'' +
+     }
+     {\verb+ st =[ while b do c end ]=> st'' +}\ (EWhileTrue)
+$$
+
+```coq
+Reserved Notation
+         "st '=[' c ']=>' st'"
+         (at level 40, c custom com at level 99,
+          st constr, st' constr at next level).
+Inductive ceval : com -> state -> state -> Prop :=
+    | E_Skip : forall st,
+        st =[ skip ]=> st
+    | E_Asgn : forall st a n x,
+        aeval st a = n ->
+        st =[ x := a ]=> (x !-> n ; st)
+    | E_Seq : forall c1 c2 st st' st'',
+        st =[ c1 ]=> st' ->
+        st' =[ c2 ]=> st'' ->
+        st =[ c1 ; c2 ]=> st''
+    | E_IfTrue : forall st st' b c1 c2,
+        beval st b = true ->
+        st =[ c1 ]=> st' ->
+        st =[ if b then c1 else c2 end]=> st'
+    | E_IfFalse : forall st st' b c1 c2,
+        beval st b = false ->
+        st =[ c2 ]=> st' ->
+        st =[ if b then c1 else c2 end]=> st'
+    | E_WhileFalse : forall b st c,
+        beval st b = false ->
+        st =[ while b do c end ]=> st
+    | E_WhileTrue : forall st st' st'' b c,
+        beval st b = true ->
+        st =[ c ]=> st' ->
+        st' =[ while b do c end ]=> st'' ->
+        st =[ while b do c end ]=> st''
+    where "st =[ c ]=> st'" := (ceval c st st').
+```
+
+$$
+\frac{\displaystyle
+      \frac{\displaystyle
+        \verb+ aeval empty_st 2 = 2 +
+      }
+      {
+        \verb+ empty_st =[ X := 2 ]=> (X !-> 2) +
+      } \ (EAsgn)
+      \qquad
+      \frac{\displaystyle
+        \verb+ beval (X !-> 2) <{ X <= 1 }> = false + \qquad
+        \frac{\displaystyle
+          \verb+ aeval (X !-> 2) 4 = 4 +
+        }
+        {
+          \verb+ (X !-> 2) =[ Z := 4 ]=> (Z !-> 4; X !-> 2) +
+        } \ (EAsgn)
+      }
+      {
+        \verb+ if (X <= 1) then Y := 3 else Z := 4 end ]=> (Z !-> 4 ; X !-> 2) +
+      } \ (EIfFalse)
+     }
+     {\verb+ empty_st =[ X := 2; if (X <= 1) then Y := 3 else Z := 4 end ]=> (Z !-> 4 ; X !-> 2) +} \ (ESeq)
+$$
+
+```coq
+Example ceval_example1:
+    empty_st =[
+        X := 2;
+        if (X <= 1)
+            then Y := 3
+            else Z := 4
+        end
+    ]=> (Z !-> 4 ; X !-> 2).
+Proof.
+    apply E_Seq with (X !-> 2).
+    - apply E_Asgn. simpl. reflexivity.
+    - apply E_IfFalse.
+      + simpl. reflexivity.
+      + apply E_Asgn. simpl. reflexivity.
+Qed.
+```
+
 # 参考文献
 - SOFTWARE FOUNDATIONS VOLUME 1 - IMP, https://softwarefoundations.cis.upenn.edu/lf-current/Imp.html
 - 計算と論理, 五十嵐 淳, https://www.fos.kuis.kyoto-u.ac.jp/~igarashi/class/cal20w/
